TargetSFI/CSTest.v
@@ -2,6 +2,8 @@ Require Import TargetSFI.CS.
 Require Import TargetSFI.Machine.
 Require Import TargetSFI.MachineGen.
 Require Import Coq.Lists.List. Import ListNotations.
+Require Import Coq.NArith.BinNat.
+Require Import Coq.ZArith.BinInt.
 Require Import Coq.Logic.Decidable.
 
 From QuickChick Require Import QuickChick.
@@ -11,6 +13,7 @@ Import GenLow GenHigh.
 Set Warnings "-extraction-opaque-accessed,-extraction".
 
 Require Import CompCert.Events.
+Require Import Common.Definitions.
 
 Import CS.
 Import Env.
@@ -38,15 +41,66 @@ Proof.
   destruct st' as [[mem' pc'] gen_regs'].
   destruct (Memory.get_word mem pc) eqn:H.
   - destruct w.
-    + right. unfold not. intro H1.
-      (* TODO Learn how to write a tactic pattern here to match all the cases
-      inversion H1; try (unfold executing in H5; subst; rewrite H in H5; auto).
-      * *)
+    + right. unfold not. intro H1. inversion H1.
+      * unfold executing in H5. subst. rewrite H in H5. auto.
+      * unfold executing in H5. subst. rewrite H in H5. auto.
+      * unfold executing in H6. subst. rewrite H in H6. auto.
+      * unfold executing in H7. subst. rewrite H in H7. auto.
+      * unfold executing in H7. subst. rewrite H in H7. auto.
+      * unfold executing in H7. subst. rewrite H in H7. auto.
+      * unfold executing in H6. subst. rewrite H in H6. auto.
+      * unfold executing in H6. subst. rewrite H in H6. auto.
+      * unfold executing in H7. subst. rewrite H in H7. auto.
+      * unfold executing in H6. subst. rewrite H in H6. auto.
+      * unfold executing in H5. subst. rewrite H in H5. auto.
+      * unfold executing in H7. subst. rewrite H in H7. auto.
+    + destruct t0.
+      * destruct (N.eqb pc' (inc_pc pc)) eqn:Hpc. rewrite N.eqb_eq in Hpc.
+        rewrite Hpc. destruct (gen_regs = gen_regs') eqn:Hregs.
+        left. apply Nop.
       Admitted.
 
-Definition trace_checker (t1 t2 : trace) : Checker := checker true. (* TODO *)
+Definition eqb_event (e1 e2: event) : bool :=
+  match (e1,e2) with
+  | (ECall c1 p1 a1 c1', ECall c2 p2 a2 c2') => (Component.eqb c1 c2)
+                                                && (Procedure.eqb p1 p2)
+                                                && (Z.eqb a1 a2)
+                                                && (Component.eqb c1' c2')
+  | (ERet c1 a1 c1', ERet c2 a2 c2') => (Component.eqb c1 c2)
+                                        (* && (Z.eqb a1 a2) *) (* the return value should not be considered *)
+                                        && (Component.eqb c1' c2')
+  | _ => false
+  end.
 
-Definition state_checker (s1 s2: MachineState.t) : Checker := checker true. (* TODO *)
+Definition trace_checker (t1 t2 : trace) : Checker :=
+  let fix aux l1 l2 :=
+      match (l1,l2) with
+      | (nil,nil) => true
+      | (e1::l1',e2::l2') => if (eqb_event e1 e2)
+                             then aux l1' l2'
+                             else false
+      | _ => false
+      end in checker (aux t1 t2).
+
+Definition eqb_regs (regs1 regs2 : RegisterFile.t) : bool :=
+    let fix aux l1 l2 :=
+      match (l1,l2) with
+      | (nil,nil) => true
+      | (r1::l1',r2::l2') => if (Z.eqb r1 r2)
+                             then aux l1' l2'
+                             else false
+      | _ => false
+      end in (aux regs1 regs2).
+
+Definition eqb_mem (mem1 mem2 : Memory.t) : bool :=
+  Memory.equal mem1 mem2.
+
+Definition state_checker (s1 s2: MachineState.t) : Checker :=
+  checker (
+      (N.eqb (MachineState.getPC s1) (MachineState.getPC s2))
+        && (eqb_regs (MachineState.getRegs s1) (MachineState.getRegs s2))
+        && (eqb_mem (MachineState.getMemory s1) (MachineState.getMemory s2))
+    ).
 
 Definition eval_step_complete_exec : Checker :=
   forAll genEnv (fun g =>
@@ -87,6 +141,6 @@ What do I need to generate?
  *)
 (* I need the Prop to be decidable. *)
 
-(* QuickChick eval_step_complete. *)
+QuickChick eval_step_complete_exec. 
                                    
   
